

Trabalho 1 de Cálculo 2

Alexandre Okamoto

Larissa Maruyama

Luisa Landert

Mikael Shin

21/10/2019

Ex 1: $\int \log(x) \, dx$

$$f' = 1, \quad f = x, \quad g = \log(x), \quad g' = \frac{1}{x}$$

$$\int \log(x) dx = \int 1 \cdot \log(x) dx$$

$$= x \cdot \log x - \int x \cdot \frac{1}{x} dx$$

$$= x \cdot \log x - x$$

$$= x(\log x - 1).$$

Ex 2: $\int x \cdot \log(x) \, dx$

$$f' = x, \quad f = \frac{x^2}{2}, \quad g = \log(x), \quad g' = \frac{1}{x}$$

$$\int x \cdot \log(x) \, dx = \frac{x^2}{2} \cdot \log x - \int \frac{x^2}{2} \cdot \frac{1}{x} \, dx$$

$$= \frac{x^2}{2} \cdot \log x - \frac{1}{2} \cdot \int x \, dx$$

$$= \frac{x^2}{2} \cdot \log x - \frac{1}{2} \cdot \frac{x^2}{2}$$

$$= \frac{x^2}{2} \cdot \left(\log x - \frac{1}{2} \right).$$

Ex 3: $\int x^n \cdot \log(x) \, dx$

$$f' = x^n, \quad f = \frac{x^{n+1}}{n+1}, \quad g = \log x, \quad g' = \frac{1}{x}$$

$$\int x^n \cdot \log(x) \, dx = \frac{x^{n+1}}{n+1} \cdot \log x - \int \frac{x^{n+1}}{n+1} \cdot \frac{1}{x} \, dx$$

$$= \frac{x^{n+1}}{n+1} \cdot \log x - \int \frac{x^n}{n+1} \, dx$$

$$= \frac{x^{n+1}}{n+1} \cdot \log x - \frac{1}{n+1} \cdot \int x^n \, dx$$

$$= \frac{x^{n+1}}{n+1} \cdot \log x - \frac{1}{n+1} \cdot \frac{x^{n+1}}{n+1}$$

$$= \frac{x^{n+1}}{n+1} \cdot \left(\log x - \frac{1}{n+1} \right).$$

Ex 4: $\int x \cdot \log(1+x) \, dx$

$$f' = x, \quad f = \frac{x^2}{2}, \quad g = \log(1+x), \quad g' = \frac{1}{x+1}$$

$$\int x \cdot \log(1+x) \, dx = \frac{x^2}{2} \cdot \log(1+x) - \int \frac{x^2}{2} \cdot \frac{1}{x+1} \, dx$$

$$= \frac{x^2}{2} \cdot \log(1+x) - \frac{1}{2} \cdot \int \frac{x^2}{1+x} \, dx$$

$$= \frac{x^2}{2} \cdot \log(1+x) - \frac{1}{2} \cdot \left[\frac{(x-1)^2}{2} + \log(1+x) \right]$$

$$= \frac{x^2}{2} \cdot \log(1+x) - \frac{(x-1)^2}{4} - \frac{1}{2} \log(1+x)$$

$$= \frac{x^2-1}{2} \cdot \log(1+x) - \frac{(x-1)^2}{4}.$$

obs: $\int \frac{x^2}{x-1}$: Referência usada pelo Ex 6.

Ex 5: $\int x \cdot \log(1-x) \, dx$

$$f' = x, \quad f = \frac{x^2}{2}, \quad g = \log(1-x), \quad g' = -\frac{1}{1-x}$$

$$\begin{aligned} \int x \cdot \log(1-x) \, dx &= \frac{x^2}{2} \cdot \log(1-x) - \int \frac{x^2}{2} \cdot \left(-\frac{1}{x-1}\right) \, dx \\ &= \frac{x^2}{2} \cdot \log(1-x) + \frac{1}{2} \cdot \int \frac{x^2}{1-x} \, dx \\ &= \frac{x^2}{2} \cdot \log(1-x) + \frac{1}{2} \cdot \left[-\frac{(x+1)^2}{2} - \log(1-x) \right] \\ &= \frac{x^2}{2} \cdot \log(1-x) - \frac{(x+1)^2}{4} - \frac{1}{2} \log(1-x) \\ &= \frac{x^2-1}{2} \cdot \log(1-x) - \frac{(1+x)^2}{4}. \end{aligned}$$

obs: $\int \frac{x^2}{x-1}$: Referência usada pelo Ex 7.

Ex 6: $\int \frac{x^2}{1+x} \, dx$

$$u = 1+x, \quad du = dx, \quad x^2 = (u-1)^2,$$

$$\begin{aligned} \int \frac{x^2}{1+x} \, dx &= \int \frac{(u-1)^2}{u} \, du \\ &= \int \frac{u^2 - 2u + 1}{u} \, du \\ &= \int u + \frac{1}{u} - 2 \, du \\ &= \int u \, du + \int \frac{1}{u} \, du - 2 \cdot \int 1 \, du \\ &= \frac{u^2}{2} + \log u - 2 \cdot u \end{aligned}$$

$$= \frac{(1+x)^2}{2} + \log(1+x) - 2 \cdot (1+x)$$

$$= \frac{1+2x+x^2}{2} - 2 - 2x + \log(1+x)$$

$$= \log(1+x) + \frac{x^2}{2} - x + C$$

$$= \log(1+x) + \frac{(x-1)^2}{2}.$$

Ex 7: $\int \frac{x^2}{1-x} dx$

$$u = 1 - x, \quad du = -dx, \quad x^2 = (1-u)^2,$$

$$\int \frac{x^2}{1-x} dx = - \int \frac{(1-u)^2}{u} du$$

$$= - \int \frac{u^2 - 2u + 1}{u} du$$

$$= - \left(\int u du - 2 \cdot \int 1 du + \int \frac{1}{u} du \right)$$

$$= - \frac{u^2}{2} - \log u + 2 \cdot u$$

$$= - \log(1-x) - \frac{(1-x)^2}{2} + 2 \cdot (1-x)$$

$$= - \log(1-x) - \left(\frac{x^2 - 2x + 1}{2} \right) + (2 - 2x)$$

$$= - \log(1-x) - \frac{x^2}{2} + x - \frac{1}{2} + 2 - 2x$$

$$= - \log(1-x) - \frac{x^2}{2} - x + C$$

$$= - \log(1-x) - \frac{(x-1)^2}{2}.$$

Ex 8: $\int \log(1+x) \, dx$

$$u = 1+x, \quad du = dx, \quad f = u, \quad f' = 1, \quad g = \log(u), \quad g' = \frac{1}{u}$$

$$\begin{aligned} \int \log(1+x) \, dx &= \int \log(u) \, du \\ &= \int 1 \cdot \log u \, du \\ &= u \cdot \log u - \int u \cdot \frac{1}{u} \, du \\ &= u \cdot \log u - \int 1 \, du \\ &= u \cdot \log u - u \\ &= (1+x) \cdot \log(1+x) - (1+x) \\ &= (1+x) \cdot \log(1+x) - x. \end{aligned}$$

Ex 9: $\int \log(1-x) \, dx$

$$u = 1-x, \quad du = -dx, \quad f = u, \quad f' = 1, \quad g = \log(u), \quad g' = \frac{1}{u}$$

$$\begin{aligned} \int \log(1-x) \, dx &= - \int \log(u) \, du \\ &= - \int 1 \cdot \log u \, du \\ &= - \left(u \cdot \log u - \int u \cdot \frac{1}{u} \, du \right) \\ &= - \left(u \cdot \log u - \int 1 \, du \right) \\ &= -u \cdot \log u + u \\ &= -(1+x) \cdot \log(1-x) + (1-x) \\ &= -(1+x) \cdot \log(1-x) - x. \end{aligned}$$

Ex 10: $\int \log(1+x^2) \, dx$

$$f = x, \quad f' = 1, \quad g = \log(1+x^2), \quad g' = \frac{1}{1+x^2} \cdot 2x$$

$$\int \log(1+x^2) \, dx = x \cdot \log(1+x^2) - \int x \cdot \frac{2x}{1+x^2} \, dx$$

$$= x \cdot \log(1+x^2) - \int \frac{2x^2}{1+x^2} \, dx$$

$$= x \cdot \log(1+x^2) - 2 \cdot \int \frac{x^2}{1+x^2} \, dx$$

$$= x \cdot \log(1+x^2) - 2 \cdot \int \frac{x^2}{1+x^2} + \frac{1+x^2}{1+x^2} - \frac{1+x^2}{1+x^2} \, dx$$

$$= x \cdot \log(1+x^2) - 2 \cdot \left[\int \frac{1+x^2}{1+x^2} \, dx - \int \frac{1}{1+x^2} \, dx \right]$$

$$= x \cdot \log(1+x^2) - 2 \cdot (x - \arctan x).$$

Ex 11: $\int \arctan(x) \, dx$

$$f = x, \quad f' = 1, \quad g = \arctan x, \quad g' = \frac{1}{1+x^2}$$

$$\int \arctan(x) \, dx = x \cdot \arctan x - \int \frac{x}{x^2+1} \, dx$$

$$= x \cdot \arctan x - \int \frac{x}{x^2+1} \, dx$$

$$u = x^2 + 1, \quad du = 2x \, dx$$

$$= x \cdot \arctan x - \int \frac{x}{u} \cdot \frac{1}{2x} \, du$$

$$= x \cdot \arctan x - \frac{1}{2} \cdot \int \frac{1}{u} \, du$$

$$= x \cdot \arctan x - \frac{1}{2} \cdot \log u$$

$$= x \cdot \arctan x - \frac{1}{2} \cdot \log(x^2 + 1).$$

Ex 12: $2 \int x \operatorname{arctg}(x) dx$

$$f = \frac{x^2}{2}, \quad f' = x, \quad g = \operatorname{arctg} x, \quad g' = \frac{1}{x^2 + 1}$$

$$\int x \operatorname{arctg}(x) dx = 2 \cdot \left[\frac{x^2 \operatorname{arctg} x}{2} - \int \frac{x^2}{2 \cdot (x^2 + 1)} dx \right]$$

$$= x^2 \operatorname{arctg} x - \int \frac{x^2}{x^2 + 1} dx$$

$$= x^2 \operatorname{arctg} x - \int \frac{x^2 + 1 - 1}{x^2 + 1} dx$$

$$= x^2 \operatorname{arctg} x - \int 1 - \frac{1}{x^2 + 1} dx$$

$$= x^2 \operatorname{arctg} x - \int 1 + \int \frac{1}{x^2 + 1} dx$$

$$= x^2 \operatorname{arctg} x - x + \operatorname{arctg} x.$$

Ex 13: $\int \sqrt{\operatorname{tg}(x)} dx$

Resolução 1:

$$u = \sqrt{\operatorname{tg} x}, \quad u^2 = \operatorname{tg} x, \quad 2 du = \frac{1}{\cos^2 x} dx = (1 + \operatorname{tg}^2 x) = (1 + u^4), \quad dx = \frac{2u}{1 + u^4} du$$

$$\int \sqrt{\operatorname{tg}(x)} dx = \int u \cdot \frac{2u}{1 + u^4} du$$

$$= \int \frac{2u^2}{1 + u^4}$$

obs*: $1 + u^4 = (u^2 + i)(u^2 - i)$

$$\frac{2u^2}{1 + u^4} = \frac{1}{(u^2 + i)} + \frac{1}{(u^2 - i)}$$

$$u^2 + i = (u + i\sqrt{i})(u - i\sqrt{i}) \quad u^2 - i = (u + \sqrt{i})(u - \sqrt{i})$$

$$\int \sqrt{\operatorname{tg}(x)} dx = \int \frac{1}{u^2 + i} + \int \frac{1}{u^2 - i} du$$

$$= \int \frac{1}{u^2 + i} du + \int \frac{1}{u^2 - i} du$$

$$\begin{aligned}
\int \frac{1}{u^2 + i} du &= \int \frac{1}{(u + i\sqrt{i})(u - i\sqrt{i})} du \\
&= \int \frac{1}{2i\sqrt{i}} \left(\frac{1}{u - i\sqrt{i}} - \frac{1}{u + i\sqrt{i}} \right) du \\
&= \frac{1}{2i\sqrt{i}} \int \left(\frac{1}{u - i\sqrt{i}} - \frac{1}{u + i\sqrt{i}} \right) du \\
&= \frac{1}{2i\sqrt{i}} \left(\int \frac{1}{u - i\sqrt{i}} du - \int \frac{1}{u + i\sqrt{i}} du \right) \\
&= \frac{1}{2i\sqrt{i}} \left[\log(u - i\sqrt{i}) - \log(u + i\sqrt{i}) \right] \\
&= \frac{1}{2i\sqrt{i}} \cdot \log \frac{u - i\sqrt{i}}{u + i\sqrt{i}}
\end{aligned}$$

$$\begin{aligned}
\int \frac{1}{u^2 - i} du &= \int \frac{1}{(u + \sqrt{i})(u - \sqrt{i})} du \\
&= \int \frac{1}{2\sqrt{i}} \left(\frac{1}{u - \sqrt{i}} - \frac{1}{u + i\sqrt{i}} \right) du \\
&= \frac{1}{2\sqrt{i}} \left(\int \frac{1}{u - \sqrt{i}} du - \int \frac{1}{u + i\sqrt{i}} du \right) \\
&= \frac{1}{2\sqrt{i}} \left[\log(u - \sqrt{i}) - \log(u + \sqrt{i}) \right] \\
&= \frac{1}{2\sqrt{i}} \cdot \log \frac{u - \sqrt{i}}{u + \sqrt{i}}
\end{aligned}$$

$$\begin{aligned}
\int \frac{1}{u^2 + i} du + \int \frac{1}{u^2 - i} du &= \left(\frac{1}{2i\sqrt{i}} \cdot \log \frac{u - i\sqrt{i}}{u + i\sqrt{i}} \right) + \left(\frac{1}{2\sqrt{i}} \cdot \log \frac{u - \sqrt{i}}{u + \sqrt{i}} \right) \\
&= \frac{1}{2i\sqrt{i}} \cdot \log \frac{\sqrt{\operatorname{tg} x} - i\sqrt{i}}{\sqrt{\operatorname{tg} x} + i\sqrt{i}} + \frac{1}{2\sqrt{i}} \cdot \log \frac{\sqrt{\operatorname{tg} x} - \sqrt{i}}{\sqrt{\operatorname{tg} x} + \sqrt{i}}.
\end{aligned}$$

Resolução 2:

$$u = \sqrt{\operatorname{tg} x}, \quad u^2 = \operatorname{tg} x, \quad dx = \frac{2u}{1 + u^4} du$$

$$\int \sqrt{\operatorname{tg}(x)} \, dx = \int u \cdot \frac{2u}{1+u^4} \, du$$

$$= \int \frac{2u^2}{1+u^4}$$

$$= 2 \int \frac{u^2}{1+u^4}$$

$$\text{obs 1 : } 1+u^4 = (u^2 - \sqrt{2}u + 1)(u^2 + \sqrt{2}u + 1)$$

$$\text{obs 2 : } \frac{1}{2\sqrt{2}} \left(\frac{u}{u^2 - \sqrt{2}u + 1} - \frac{u}{u^2 + \sqrt{2}u + 1} \right)$$

$$\text{obs 3 : } \int \frac{u}{u^2 - \sqrt{2}u + 1} \, du = \frac{1}{2} \int \frac{2u - \sqrt{2} + \sqrt{2}}{u^2 - \sqrt{2}u + 1} \, du = \frac{1}{2} \left[\log(u^2 - \sqrt{2}u + 1) + \sqrt{2} \int \frac{1}{u^2 - \sqrt{2}u + 1} \, du \right]$$

$$\int \sqrt{\operatorname{tg}(x)} \, dx = \frac{2}{2\sqrt{2}} \int \left(\frac{u}{u^2 - \sqrt{2}u + 1} - \frac{u}{u^2 + \sqrt{2}u + 1} \right) \, du$$

$$= \frac{2}{2\sqrt{2}} \left[\frac{1}{2} \log(u^2 - \sqrt{2}u + 1) + \operatorname{arc\,tg}(\sqrt{2}u - 1) \right]$$

$$= \frac{2}{2\sqrt{2}} \left[\frac{1}{2} \log(\sqrt{\operatorname{tg} x}^2 - \sqrt{2} \cdot \sqrt{\operatorname{tg} x} + 1) + \operatorname{arc\,tg}(\sqrt{2} \cdot \sqrt{\operatorname{tg} x} - 1) \right]$$

$$= \frac{2}{2\sqrt{2}} \left[\frac{1}{2} \log(\operatorname{tg} x - \sqrt{2} \operatorname{tg} x + 1) + \operatorname{arc\,tg}(\sqrt{2} \operatorname{tg} x - 1) \right].$$

Resolução 3:

$$u = \sqrt{\operatorname{tg} x}, \quad \frac{du}{dx} = \frac{1}{2\sqrt{\operatorname{tg} x} \cos^2 x}$$

$$\int \sqrt{\operatorname{tg}(x)} \, dx = \int \frac{2u^2}{u^4 + 1} \, du$$

$$u^2 = iy^2, \quad du = \sqrt{i} \, dy, \quad u^4 = -y^4$$

$$= \int \frac{2iy^2}{-y^4 + 1} \cdot \sqrt{i} \, dy$$

$$= 2i\sqrt{i} \int \frac{y^2}{1 - y^4} \, dy$$

$$= 2i\sqrt{i} \int \frac{1}{2} \left(\frac{y^2}{1-y^2} + \frac{y^2}{1+y^2} \right) dy$$

$$= i\sqrt{i} \int \left(\frac{y^2}{1-y^2} + \frac{y^2}{1+y^2} \right) dy$$

$$= i\sqrt{i} \int \frac{y^2}{1-y^2} dy + \int \frac{y^2}{1+y^2} dy$$

$$= i\sqrt{i} \left(-y + \frac{1}{2} \log \frac{1+y}{1-y} + y - \arctg y \right)$$

$$= i\sqrt{i} \left(\frac{1}{2} \log \frac{1+y}{1-y} - \arctg y \right)$$

$$y = \frac{\sqrt{i}\sqrt{\operatorname{tg} x}}{i}$$

$$= i\sqrt{i} \left(\frac{1}{2} \log \frac{1 + \frac{\sqrt{i}\sqrt{\operatorname{tg} x}}{i}}{1 - \frac{\sqrt{i}\sqrt{\operatorname{tg} x}}{i}} - \arctg \frac{\sqrt{i}\sqrt{\operatorname{tg} x}}{i} \right).$$